Optimization working

Source/DafnyStandardLibraries/src/Std/Actions/BulkActions.dfy
@@ -5,8 +5,10 @@ module Std.BulkActions {
   import opened Producers
   import opened Wrappers
   import opened BoundedInts
+  import opened Termination
 
-  datatype OptionResult<T, E> = Good(value: T) | Bad(error: E) | Done
+  type StreamedValue<T, E> = Option<Result<T, E>>
+  type StreamedByte<E> = Option<Result<uint8, E>>
 
   @AssumeCrossModuleTermination
   trait BulkAction<I, O> extends Action<I, O> {
@@ -24,17 +26,142 @@ module Std.BulkActions {
       ensures input.Valid()
       ensures output.Valid()
   }
+  
+  /**
+   * The equivalent of MappedProducer(ToOptionResult, original),
+   * but a separate class so it's possible to optimize via "is" testing.
+   */
+  @AssumeCrossModuleTermination
+  class BatchProducer<T, E> extends Producer<StreamedValue<T, E>> {
 
-  // @AssumeCrossModuleTermination
-  // class SeqOfResultReader<T, E> extends Producer<Result<T, E>> {
+    const elements: seq<T>
+    var index: nat
 
-  //   const r: Result<seq<T>, E>
+    constructor(elements: seq<T>)
+      ensures Valid()
+      ensures history == []
+      ensures fresh(Repr)
+      reads {}
+      ensures this.elements == elements
+      ensures index == 0
+    {
+      this.elements := elements;
+      this.index := 0;
 
+      Repr := {this};
+      history := [];
+    }
 
+    ghost predicate Valid()
+      reads this, Repr
+      ensures Valid() ==> this in Repr
+      ensures Valid() ==> ValidHistory(history)
+      decreases Repr, 0
+    {
+      && this in Repr
+      && ValidHistory(history)
+      && (Done() ==> index == |elements|)
+      && index <= |elements|
+      && Produced() == Seq.Map(ToOptionResult, elements[..index])
+      && (index < |elements| ==> Seq.All(Outputs(), IsSome))
+    }
 
-  // }
+    ghost predicate ValidOutputs(outputs: seq<Option<StreamedValue<T, E>>>)
+      requires Seq.Partitioned(outputs, IsSome)
+      decreases Repr
+    {
+      true
+    }
 
-  class Chunker<E> extends BulkAction<Option<Result<uint8, E>>, Producer<Option<Result<uint8, E>>>> {
+    ghost function RemainingMetric(): TerminationMetric
+      requires Valid()
+      reads this, Repr
+      decreases Repr, 3
+    {
+      TMNat(|elements| - index)
+    }
+
+    @IsolateAssertions
+    method Invoke(t: ()) returns (value: Option<StreamedValue<T, E>>)
+      requires Requires(t)
+      reads Reads(t)
+      modifies Modifies(t)
+      decreases Decreases(t), 0
+      ensures Ensures(t, value)
+      ensures RemainingDecreasedBy(value)
+    {
+      assert Requires(t);
+      assert Valid();
+      reveal TerminationMetric.Ordinal();
+
+      if |elements| == index {
+        value := None;
+
+        OutputsPartitionedAfterOutputtingNone();
+        ProduceNone();
+      } else {
+        value := Some(Some(Success(elements[index])));
+
+        OutputsPartitionedAfterOutputtingSome(value.value);
+        ProduceSome(value.value);
+        index := index + 1;
+      }
+
+      assert Valid();
+    }
+
+    // TODO: Use this in an override of ForEachRemaining(seq consumer)
+    @IsolateAssertions
+    method Read() returns (s: seq<T>)
+      requires Valid()
+      reads this, Repr
+      modifies Repr
+      ensures ValidAndDisjoint()
+      ensures Done()
+    {
+      // Avoid the slice if possible
+      if index == 0 {
+        s := elements;
+      } else {
+        s := elements[index..];
+      }
+      index := |elements|;
+
+      var produced := Seq.Map(ToOptionResult, s);
+      var outputs := OutputsForProduced(produced, |s| + 1);
+      history := history + Seq.Zip(Seq.Repeat((), |s| + 1), outputs);
+      assert Seq.Last(Outputs()) == None;
+      assert Outputs() == old(Outputs()) + outputs;
+      if |s| == 0 {
+        assert Seq.AllNot(outputs, IsSome);
+        Seq.PartitionedCompositionRight(old(Outputs()), outputs, IsSome);
+      } else {
+        assert Seq.All(old(Outputs()), IsSome);
+        Seq.PartitionedCompositionLeft(old(Outputs()), outputs, IsSome);
+      }
+      ProducedComposition(old(Outputs()), outputs);
+      
+      assert Valid();
+    }
+
+  }
+
+  function ToOptionResult<T, E>(t: T): Option<Result<T, E>> {
+    Some(Success(t))
+  }
+
+  method ToOptionResultProducer<T, E>(values: seq<T>) returns (result: Producer<Option<Result<T, E>>>)
+    reads {}
+    ensures result.Valid()
+    ensures fresh(result.Repr)
+    ensures result.history == []
+  {
+    var chunkProducer := new SeqReader(values);
+    var mapping := new FunctionAction(ToOptionResult);
+    var mappingTotalProof := new TotalFunctionActionProof(mapping);
+    result := new MappedProducer(chunkProducer, mapping, mappingTotalProof);
+  }
+  class Chunker<E> extends BulkAction<StreamedByte<E>, Producer<StreamedByte<E>>> {
 
     const chunkSize: uint64
     var chunkBuffer: BoundedInts.bytes
@@ -61,13 +188,13 @@ module Std.BulkActions {
       && 0 < chunkSize
     }
 
-    ghost predicate ValidHistory(history: seq<(Option<Result<uint8, E>>, Producer<Option<Result<uint8, E>>>)>)
+    ghost predicate ValidHistory(history: seq<(StreamedByte<E>, Producer<StreamedByte<E>>)>)
       decreases Repr
     {
       true
     }
 
-    ghost predicate ValidInput(history: seq<(Option<Result<uint8, E>>, Producer<Option<Result<uint8, E>>>)>, next: Option<Result<uint8, E>>)
+    ghost predicate ValidInput(history: seq<(StreamedByte<E>, Producer<StreamedByte<E>>)>, next: StreamedByte<E>)
       requires ValidHistory(history)
       decreases Repr
     {
@@ -96,57 +223,49 @@ module Std.BulkActions {
       0
     }
 
-    method Invoke(i: Option<Result<uint8, E>>) returns (o: Producer<Option<Result<uint8, E>>>)
+    @ResourceLimit("0")
+    method Invoke(i: StreamedByte<E>) returns (o: Producer<StreamedByte<E>>)
       requires Requires(i)
-      reads Reads(i)
+      reads this, Repr
       modifies Modifies(i)
       decreases Decreases(i), 0
       ensures Ensures(i, o)
     {
+      assert Valid();
       var input := new SeqReader([i]);
       var output := new SeqWriter();
       var outputTotalProof := new SeqWriterTotalActionProof(output);
       BulkInvoke(input, output, outputTotalProof);
+      assert input.Valid();
+      assert |output.values| == 1;
       o := output.values[0];
+
+      assert input.Produced() == [i];
+      assert Inputs() == old(Inputs()) + [i];
+      assert Outputs() == old(Outputs()) + [o];
     }
 
     
-    function ToOptionResult<T, E>(t: T): Option<Result<T, E>> {
-      Some(Success(t))
-    }
 
-    method ToOptionResultProducer<T, E>(values: seq<T>) returns (result: Producer<Option<Result<T, E>>>)
-      reads {}
-      ensures result.Valid()
-      ensures fresh(result.Repr)
-      ensures result.history == []
-    {
-      var chunkProducer := new SeqReader(values);
-      var mapping := new FunctionAction(ToOptionResult);
-      var mappingTotalProof := new TotalFunctionActionProof(mapping);
-      result := new MappedProducer(chunkProducer, mapping, mappingTotalProof);
-    }
-
-    // TODO: Consider dedicated three-state datatype instead of Option<Result<...>>
-    // Result is all values produced, plus the terminal state: 
+    // Result is all values produced, plus the terminal state:
     // normal (Success(true)), EOI (Success(false)) or error (Failure(error))
+    // TODO: Consider dedicated three-state datatype instead of Option<Result<...>>
+    // TODO: Make this an implementation of AcceptAll() for a kind of Consumer?
     method CollectToSeqResult<T, E>(p: Producer<Option<Result<T, E>>>) returns (values: seq<T>, state: Result<bool, E>)
       requires p.Valid()
       reads p, p.Repr
       modifies p.Repr
       ensures p.ValidAndDisjoint()
       ensures p.Done()
-
+      // TODO: ensures relationship between p.Produced() and values/state
     {
-      // TODO: optimization - needs duplicate class to get around lack of compiled is
-      // if p is MappedProducer<T, Option<Result<T, E>>> {
-      //   var mp := p as MappedProducer;
-      //   if mp.mapping is FunctionAction<T, Option<Result<T, E>>> {
-      //     values := CollectToSeq(mp.original);
-      //     state := Success(true);
-      //     return;
-      //   }
-      // }
+      // Optimization
+      if p is BatchProducer<T, E> {
+        var bp := p as BatchProducer<T, E>;
+        values := bp.Read();
+        state := Success(true);
+        return;
+      }
 
       values := [];
       state := Success(true);
@@ -172,9 +291,9 @@ module Std.BulkActions {
     }
 
     @ResourceLimit("0")
-    method BulkInvoke(input: Producer<Option<Result<uint8, E>>>, 
-                      output: IConsumer<Producer<Option<Result<uint8, E>>>>,
-                      outputTotalProof: TotalActionProof<Producer<Option<Result<uint8, E>>>, ()>)
+    method BulkInvoke(input: Producer<StreamedByte<E>>, 
+                      output: IConsumer<Producer<StreamedByte<E>>>,
+                      outputTotalProof: TotalActionProof<Producer<StreamedByte<E>>, ()>)
       requires Valid()
       requires input.Valid()
       requires output.Valid()
@@ -183,9 +302,12 @@ module Std.BulkActions {
       requires Repr !! input.Repr !! output.Repr !! outputTotalProof.Repr
       reads this, Repr, input, input.Repr, output, output.Repr, outputTotalProof, outputTotalProof.Repr
       modifies Repr, input.Repr, output.Repr, outputTotalProof.Repr
-      ensures Valid()
-      ensures input.Valid()
-      ensures output.Valid()
+      ensures ValidAndDisjoint()
+      ensures input.ValidAndDisjoint()
+      ensures output.ValidAndDisjoint()
+      ensures input.Done()
+      ensures Inputs() == input.Produced()
+      ensures Outputs() == output.Inputs()
     {
       assert Valid();
 
@@ -197,6 +319,7 @@ module Std.BulkActions {
         invariant Valid()
         invariant fresh(input.Repr - old(input.Repr))
         invariant input.Valid()
+        invariant input.Done()
         invariant fresh(output.Repr - old(output.Repr))
         invariant output.Valid()
         invariant fresh(outputTotalProof.Repr - old(outputTotalProof.Repr))
@@ -228,6 +351,8 @@ module Std.BulkActions {
         }
       case Success(true) => {}
       }
+
+      history := history + Seq.Zip(input.Produced(), output.Inputs());
     }
   }
 
